src/lowparse/LowParse.SLow.Bytes.fst
@@ -18,95 +18,111 @@ let parse32_flbytes_gen
 
 inline_for_extraction
 let parse32_flbytes
+  (#err: Type)
   (sz: nat)
   (sz' : U32.t { U32.v sz' == sz } )
+  (e: err)
 : Tot (
      lt_pow2_32 sz;
-     parser32 (parse_flbytes sz)
+     parser32 (parse_flbytes sz e)
   )
 = lt_pow2_32 sz;
   make_total_constant_size_parser32
     sz
     sz'
     #(B32.lbytes sz)
+    #err
     (parse_flbytes_gen sz)
+    e
     ()
     (parse32_flbytes_gen sz)
 
 inline_for_extraction
 let serialize32_flbytes
+  (#err: Type0)
   (sz: nat { sz < 4294967296 } )
-: Tot (serializer32 (serialize_flbytes sz))
+  (e: err)
+: Tot (serializer32 (serialize_flbytes sz e))
 = fun (input: B32.lbytes sz) ->
     B32.hide_reveal input;
-    (input <: (res: bytes32 { serializer32_correct (serialize_flbytes sz) input res } ))
+    (input <: (res: bytes32 { serializer32_correct (serialize_flbytes sz e) input res } ))
 
 inline_for_extraction
 let parse32_all_bytes
-  : parser32 parse_all_bytes
+  (#err: Type0)
+  (e: err)
+: Tot (parser32 (parse_all_bytes e))
 = fun (input: B32.bytes) ->
-    let res = Some (input, B32.len input) in
-    (res <: (res: option (bytes32 * U32.t) { parser32_correct parse_all_bytes input res } ))
+    let res = Correct (input, B32.len input) in
+    (res <: (res: result (bytes32 * U32.t) err { parser32_correct (parse_all_bytes e) input res } ))
 
 inline_for_extraction
 let serialize32_all_bytes
-  : serializer32 serialize_all_bytes
+  (#err: Type0)
+  (e: err)
+: Tot (serializer32 (serialize_all_bytes e))
 = fun (input: B32.bytes) ->
-  (input <: (res: bytes32 { serializer32_correct serialize_all_bytes input res } ))
+  (input <: (res: bytes32 { serializer32_correct (serialize_all_bytes e) input res } ))
 
 inline_for_extraction
 let parse32_bounded_vlbytes
+  (#err: Type0)
   (min: nat)
   (min32: U32.t { U32.v min32 == min } )
   (max: nat { min <= max /\ max > 0 /\ max < 4294967296 })
   (max32: U32.t { U32.v max32 == max } )
-: Tot (parser32 (parse_bounded_vlbytes min max))
+  (e_size_incomplete e_size_invalid: err)
+: Tot (parser32 (parse_bounded_vlbytes min max e_size_incomplete e_size_invalid))
 = parse32_synth
     _
-    (synth_bounded_vlbytes min max)
-    (fun (x: parse_bounded_vldata_strong_t min max #_ #_ #parse_all_bytes serialize_all_bytes) -> (x <: parse_bounded_vlbytes_t min max))
-    (parse32_bounded_vldata_strong min min32 max max32 serialize_all_bytes parse32_all_bytes)
+    (synth_bounded_vlbytes min max e_size_invalid)
+    (fun (x: parse_bounded_vldata_strong_t min max (serialize_all_bytes e_size_invalid)) -> (x <: parse_bounded_vlbytes_t min max))
+    (parse32_bounded_vldata_strong min min32 max max32 (serialize_all_bytes e_size_invalid) (parse32_all_bytes e_size_invalid) e_size_incomplete e_size_invalid e_size_invalid)
     ()
 
 inline_for_extraction
 let serialize32_bounded_vlbytes
+  (#err: Type0)
   (min: nat)
   (max: nat { min <= max /\ max > 0 /\ max < 4294967292 } ) // max MUST BE less than 2^32 - 4
-: Tot (serializer32 (serialize_bounded_vlbytes min max))
+  (e_size_incomplete e_size_invalid: err)
+: Tot (serializer32 (serialize_bounded_vlbytes min max e_size_incomplete e_size_invalid))
 = fun (input: parse_bounded_vlbytes_t min max) ->
   serialize32_bounded_vldata_strong
     min
     max
-    #_
-    #_
-    #parse_all_bytes
-    #serialize_all_bytes
-    serialize32_all_bytes
+    (total_to_partial_serializer32 (serialize32_all_bytes e_size_invalid))
+    e_size_incomplete
+    e_size_invalid
+    e_size_invalid
     input
 
 #reset-options "--z3rlimit 32 --z3cliopt smt.arith.nl=false"
 
 inline_for_extraction
 let size32_all_bytes
-: size32 serialize_all_bytes
+  (#err: Type0)
+  (e: err)
+: Tot (size32 (serialize_all_bytes e))
 = fun (input: B32.bytes) ->
   let res = B32.len input in
-  (res <: (res: U32.t { size32_postcond serialize_all_bytes input res } ))
+  (res <: (res: U32.t { size32_postcond (serialize_all_bytes e) input res } ))
 
 inline_for_extraction
 let size32_bounded_vlbytes
+  (#err: Type0)
   (min: nat)
   (max: nat { min <= max /\ max > 0 /\ max < 4294967292 } ) // max MUST BE less than 2^32 - 4
   (size_header_byte_size32: U32.t { U32.v size_header_byte_size32 == log256' max } )
-: Tot (size32 (serialize_bounded_vlbytes min max))
+  (e_size_incomplete e_size_invalid: err)
+: Tot (size32 (serialize_bounded_vlbytes min max e_size_incomplete e_size_invalid))
 = fun (input: parse_bounded_vlbytes_t min max) ->
   size32_bounded_vldata_strong
     min
     max
-    #_
-    #_
-    #parse_all_bytes
-    #serialize_all_bytes
-    size32_all_bytes
+    (size32_all_bytes e_size_invalid)
     size_header_byte_size32
+    e_size_incomplete
+    e_size_invalid
+    e_size_invalid
     input
