src/lowparse/LowParse.SLow.Combinators.fst
@@ -10,56 +10,59 @@ module U32 = FStar.UInt32
 inline_for_extraction
 let parse32_ret
   (#t: Type)
+  (#err: Type0)
   (x: t)
 : Tot (parser32 (parse_ret x))
-= (fun input -> ((Some (x, 0ul)) <: (res: option (t * U32.t) { parser32_correct (parse_ret x) input res } )))
+= (fun input -> ((Correct (x, 0ul)) <: (res: result (t * U32.t) err { parser32_correct (parse_ret x) input res } )))
 
 inline_for_extraction
 let parse32_and_then
   (#k: parser_kind)
   (#t:Type)
-  (#p:parser k t)
+  (#err: Type0)
+  (#p:parser k t err)
   (p32: parser32 p)
   (#k': parser_kind)
   (#t':Type)
-  (p': (t -> Tot (parser k' t')))
+  (p': (t -> Tot (parser k' t' err)))
   (u: unit { and_then_cases_injective p' } )
   (p32' : ((x: t) -> Tot (parser32 (p' x))))
 : Tot (parser32 (p `and_then` p'))
 = fun (input: bytes32) ->
   ((match p32 input with
-  | Some (v, l) ->
+  | Correct (v, l) ->
     let input' = B32.slice input l (B32.len input) in
     begin match p32' v input' with
-    | Some (v', l') ->
-      Some (v', U32.add l l')
-    | _ -> None
+    | Correct (v', l') ->
+      Correct (v', U32.add l l')
+    | Error e -> Error e
     end
-  | _ -> None
-  ) <: (res: option (t' * U32.t) { parser32_correct (p `and_then` p') input res } ))
+  | Error e -> Error e
+  ) <: (res: result (t' * U32.t) err { parser32_correct (p `and_then` p') input res } ))
 
 inline_for_extraction
 let parse32_nondep_then
   (#k1: parser_kind)
   (#t1: Type0)
-  (#p1: parser k1 t1)
+  (#err: Type0)
+  (#p1: parser k1 t1 err)
   (p1' : parser32 p1)
   (#k2: parser_kind)
   (#t2: Type0)
-  (#p2: parser k2 t2)
+  (#p2: parser k2 t2 err)
   (p2' : parser32 p2)
 : Tot (parser32 (nondep_then p1 p2))
 = fun (input: bytes32) ->
   ((match p1' input with
-  | Some (v, l) ->
+  | Correct (v, l) ->
     let input' = B32.slice input l (B32.len input) in
     begin match p2' input' with
-    | Some (v', l') ->
-      Some ((v, v'), U32.add l l')
-    | _ -> None
+    | Correct (v', l') ->
+      Correct ((v, v'), U32.add l l')
+    | Error e -> Error e
     end
-  | _ -> None
-  ) <: (res: option ((t1 * t2) * U32.t) { parser32_correct (p1 `nondep_then` p2) input res } ))
+  | Error e -> Error e
+  ) <: (res: result ((t1 * t2) * U32.t) err { parser32_correct (p1 `nondep_then` p2) input res } ))
 
 let serialize32_kind_precond
   (k1 k2: parser_kind)
@@ -72,13 +75,14 @@ inline_for_extraction
 let serialize32_nondep_then
   (#k1: parser_kind)
   (#t1: Type0)
-  (#p1: parser k1 t1)
+  (#err: Type0)
+  (#p1: parser k1 t1 err)
   (#s1: serializer p1)
   (s1' : serializer32 s1)
   (u: unit { k1.parser_kind_subkind == Some ParserStrong } )
   (#k2: parser_kind)
   (#t2: Type0)
-  (#p2: parser k2 t2)
+  (#p2: parser k2 t2 err)
   (#s2: serializer p2)
   (s2' : serializer32 s2)
   (u' : unit {
@@ -97,28 +101,30 @@ inline_for_extraction
 let parse32_strengthen
   (#k: parser_kind)
   (#t1: Type0)
-  (#p1: parser k t1)
+  (#err: Type0)
+  (#p1: parser k t1 err)
   (p1' : parser32 p1)
   (p2: t1 -> GTot Type0)
   (prf: parse_strengthen_prf p1 p2)
 : Tot (parser32 (parse_strengthen p1 p2 prf))
 = fun (xbytes: bytes32) -> ((
   match p1' xbytes with
-  | Some (x, consumed) ->
+  | Correct (x, consumed) ->
     [@inline_let]
     let _ = prf (B32.reveal xbytes) (U32.v consumed) x in
     [@inline_let]
     let (x' : t1 { p2 x' } ) = x in
-    Some (x', consumed)
-  | _ -> None
-  ) <: (res: option ((x: t1 { p2 x}) * U32.t) { parser32_correct (parse_strengthen p1 p2 prf) xbytes res } ))
+    Correct (x', consumed)
+  | Error e -> Error e
+  ) <: (res: result ((x: t1 { p2 x}) * U32.t) err { parser32_correct (parse_strengthen p1 p2 prf) xbytes res } ))
 
 inline_for_extraction
 let parse32_synth
   (#k: parser_kind)
   (#t1: Type0)
   (#t2: Type0)
-  (p1: parser k t1)
+  (#err: Type0)
+  (p1: parser k t1 err)
   (f2: t1 -> GTot t2)
   (f2': (x: t1) -> Tot (y: t2 { y == f2 x } )) 
   (p1' : parser32 p1)
@@ -129,16 +135,17 @@ let parse32_synth
 = fun (input: bytes32) ->
   ((
     match p1' input with
-    | Some (v1, consumed) -> Some (f2' v1, consumed)
-    | _ -> None
-   ) <: (res: option (t2 * U32.t) { parser32_correct (parse_synth p1 f2) input res } ))
+    | Correct (v1, consumed) -> Correct (f2' v1, consumed)
+    | Error e -> Error e
+   ) <: (res: result (t2 * U32.t) err { parser32_correct (parse_synth p1 f2) input res } ))
 
 inline_for_extraction
 let serialize32_synth
   (#k: parser_kind)
   (#t1: Type0)
   (#t2: Type0)
-  (p1: parser k t1)
+  (#err: Type0)
+  (p1: parser k t1 err)
   (f2: t1 -> GTot t2)
   (s1: serializer p1)
   (s1' : serializer32 s1)
@@ -157,88 +164,73 @@ inline_for_extraction
 let parse32_filter
   (#k: parser_kind)
   (#t: Type0)
-  (#p: parser k t)
+  (#err: Type0)
+  (#p: parser k t err)
   (p32: parser32 p)
   (f: (t -> GTot bool))
+  (e: err)
   (g: ((x: t) -> Tot (b: bool { b == f x } )))
-: Tot (parser32 (parse_filter p f))
+: Tot (parser32 (parse_filter p f e))
 = fun (input: bytes32) ->
   ((
     match p32 input with
-    | Some (v, consumed) ->
+    | Correct (v, consumed) ->
       if g v
       then
         [@inline_let]
         let (v' : t { f v' == true } ) = v in
-	Some (v', consumed)
+	Correct (v', consumed)
       else
-        None
-    | _ -> None
-  ) <: (res: option ((v': t { f v' == true } ) * U32.t) { parser32_correct (parse_filter p f) input res } ))
+        Error e
+    | Error e' -> Error e'
+  ) <: (res: result ((v': t { f v' == true } ) * U32.t) err { parser32_correct (parse_filter p f e) input res } ))
 
 inline_for_extraction
 let serialize32_filter
   (#k: parser_kind)
   (#t: Type0)
-  (#p: parser k t)
+  (#err: Type0)
+  (#p: parser k t err)
   (#s: serializer p)
   (s32: serializer32 s)
   (f: (t -> GTot bool))
-: Tot (serializer32 #_ #_ #(parse_filter p f) (serialize_filter s f))
+  (e: err)
+: Tot (serializer32 (serialize_filter s f e))
 = fun (input: t { f input == true } ) -> s32 input
-
-inline_for_extraction
-let make_constant_size_parser32
-  (sz: nat)
-  (sz' : U32.t { U32.v sz' == sz } )
-  (#t: Type0)
-  (f: ((s: bytes {Seq.length s == sz}) -> GTot (option t)))
-  (u: unit {
-    make_constant_size_parser_precond sz t f
-  } )
-  (f' : ((s: B32.lbytes sz) -> Tot (y: option t { y == f (B32.reveal s) } )))
-: Tot (parser32 (make_constant_size_parser sz t f))
-= fun (input: bytes32) -> ((
-    if U32.lt (B32.len input) sz'
-    then None
-    else begin
-      let s' = B32.slice input 0ul sz' in
-      match f' s' with
-      | None -> None
-      | Some v -> Some (v, sz')
-    end
-  ) <: (res: option (t * U32.t) { parser32_correct (make_constant_size_parser sz t f) input res } ))
 
 inline_for_extraction
 let make_total_constant_size_parser32
   (sz: nat)
   (sz' : U32.t { U32.v sz' == sz } )
   (#t: Type0)
+  (#err: Type0)
   (f: ((s: bytes {Seq.length s == sz}) -> GTot (t)))
+  (e: err)
   (u: unit {
     make_total_constant_size_parser_precond sz t f
   })
   (f' : ((s: B32.lbytes sz) -> Tot (y: t { y == f (B32.reveal s) } )))
-: Tot (parser32 (make_total_constant_size_parser sz t f))
+: Tot (parser32 (make_total_constant_size_parser sz t _ f e))
 = fun (input: bytes32) -> ((
     if U32.lt (B32.len input) sz'
-    then None
+    then Error e
     else
       let s' = B32.slice input 0ul sz' in
-      Some (f' s', sz')
-  ) <: (res: option (t * U32.t) { parser32_correct (make_total_constant_size_parser sz t f) input res } ))
+      Correct (f' s', sz')
+  ) <: (res: result (t * U32.t) err { parser32_correct (make_total_constant_size_parser sz t _ f e) input res } ))
 
 inline_for_extraction
 let size32_nondep_then
   (#k1: parser_kind)
   (#t1: Type0)
-  (#p1: parser k1 t1)
+  (#err: Type0)
+  (#p1: parser k1 t1 err)
   (#s1: serializer p1)
   (s1' : size32 s1)
   (u: unit { k1.parser_kind_subkind == Some ParserStrong } )
   (#k2: parser_kind)
   (#t2: Type0)
-  (#p2: parser k2 t2)
+  (#p2: parser k2 t2 err)
   (#s2: serializer p2)
   (s2' : size32 s2)
 : Tot (size32 (serialize_nondep_then _ s1 u _ s2))
@@ -254,11 +246,13 @@ inline_for_extraction
 let size32_filter
   (#k: parser_kind)
   (#t: Type0)
-  (#p: parser k t)
+  (#err: Type0)
+  (#p: parser k t err)
   (#s: serializer p)
   (s32: size32 s)
   (f: (t -> GTot bool))
-: Tot (size32 #_ #_ #(parse_filter p f) (serialize_filter s f))
+  (e: err)
+: Tot (size32 (serialize_filter s f e))
 = fun x -> s32 x
 
 inline_for_extraction
@@ -266,7 +260,8 @@ let size32_synth
   (#k: parser_kind)
   (#t1: Type0)
   (#t2: Type0)
-  (p1: parser k t1)
+  (#err: Type0)
+  (p1: parser k t1 err)
   (f2: t1 -> GTot t2)
   (s1: serializer p1)
   (s1' : size32 s1)
