src/lowparse/LowParse.SLow.Int.Aux.fst
@@ -11,53 +11,73 @@ module B32 = LowParse.Bytes32
 
 inline_for_extraction
 let serialize32_u8
-: serializer32 serialize_u8
+  (#err: Type0)
+  (e: err)
+: Tot (serializer32 (serialize_u8 e))
 = (fun (input: U8.t) ->
     let b = B32.create 1ul input in
     B32.b32_reveal_create 1ul input;
-    (b <: (res: bytes32 { serializer32_correct #_ #_ #parse_u8 serialize_u8 input res } )))
+    (b <: (res: bytes32 { serializer32_correct (serialize_u8 e) input res } )))
 
 inline_for_extraction
-let serialize32_u16 : serializer32 #_ #_ #parse_u16 serialize_u16 =
-  (fun (input: U16.t) ->
+let serialize32_u16
+  (#err: Type0)
+  (e: err)
+: Tot (serializer32 (serialize_u16 e))
+= (fun (input: U16.t) ->
     let b = E.n_to_be_2 _ _ (E.u16 ()) input in
     assert (E.n_to_be 2ul (U16.v input) == B32.reveal b);
-    (b <: (res: B32.bytes { serializer32_correct #_ #_ #parse_u16 serialize_u16 input res } )))
+    (b <: (res: B32.bytes { serializer32_correct (serialize_u16 e) input res } )))
 
 inline_for_extraction
-let serialize32_u32 : serializer32 #_ #_ #parse_u32 serialize_u32 =
+let serialize32_u32
+  (#err: Type0)
+  (e: err)
+: Tot (serializer32 (serialize_u32 e)) =
   (fun (input: U32.t) ->
     let b = E.n_to_be_4 _ _ (E.u32 ()) input in
     assert (E.n_to_be 4ul (U32.v input) == B32.reveal b);
-    (b <: (res: B32.bytes { serializer32_correct #_ #_ #parse_u32 serialize_u32 input res } )))
+    (b <: (res: B32.bytes { serializer32_correct (serialize_u32 e) input res } )))
 
 inline_for_extraction
-let parse32_u16 : parser32 parse_u16 =
-  decode_u16_injective ();
+let parse32_u16
+  (#err: Type0)
+  (e: err)
+: Tot (parser32 (parse_u16 e))
+=   decode_u16_injective ();
     make_total_constant_size_parser32 2 2ul
       #U16.t
       decode_u16
+      e
       ()
       (fun (input: B32.lbytes 2) ->
         let res = E.be_to_n_2 _ _ (E.u16 ()) input in
         (res <: (res: U16.t { res == decode_u16 (B32.reveal input) } )))
 
 inline_for_extraction
-let parse32_u32 : parser32 parse_u32 =
-    decode_u32_injective ();
+let parse32_u32
+  (#err: Type0)
+  (e: err)
+: Tot (parser32 (parse_u32 e))
+=   decode_u32_injective ();
     make_total_constant_size_parser32 4 4ul
       #U32.t
       decode_u32
+      e
       ()
       (fun (input: B32.lbytes 4) ->
         let res = E.be_to_n_4 _ _ (E.u32 ()) input in
         (res <: (res: U32.t { res == decode_u32 (B32.reveal input) } )))
 
 inline_for_extraction
-let parse32_u8 : parser32 parse_u8 =
-  decode_u8_injective ();
+let parse32_u8
+  (#err: Type0)
+  (e: err)
+: Tot (parser32 (parse_u8 e))
+= decode_u8_injective ();
   make_total_constant_size_parser32 1 1ul
     decode_u8
+    e
     ()
     (fun (b: B32.lbytes 1) ->
       let r = B32.get b 0ul in
