src/lowparse/LowParse.SLow.Int.fst
@@ -8,56 +8,53 @@ module U16 = FStar.UInt16
 module U32 = FStar.UInt32
 module B32 = FStar.Bytes
 
-let parse32_u8 =
+let parse32_u8 #err e =
   (fun input ->
     [@inline_let]
-    let _ = Unique.parse_u8_unique (B32.reveal input) in
+    let _ = Unique.parse_u8_unique e (B32.reveal input) in
     [@inline_let]
-    let res : option (U8.t * U32.t) = Aux.parse32_u8 input in
-    (res <: (res: option (U8.t * U32.t) { parser32_correct parse_u8 input res } ))
+    let res : result (U8.t * U32.t) err = Aux.parse32_u8 e input in
+    (res <: (res: result (U8.t * U32.t) err { parser32_correct (parse_u8 e) input res } ))
   )
 
-let serialize32_u8
-: serializer32 serialize_u8
-= (fun (input: U8.t) ->
+let serialize32_u8 #err e =
+  (fun (input: U8.t) ->
     [@inline_let]
-    let _ = Unique.serialize_u8_unique input in
+    let _ = Unique.serialize_u8_unique e input in
     [@inline_let]
-    let res : bytes32 = Aux.serialize32_u8 input in
-    (res <: (res: bytes32 { serializer32_correct #_ #_ #parse_u8 serialize_u8 input res } )))
+    let res : bytes32 = Aux.serialize32_u8 e input in
+    (res <: (res: bytes32 { serializer32_correct (serialize_u8 e) input res } )))
 
-let parse32_u16 =
+let parse32_u16 #err e =
   (fun input ->
     [@inline_let]
-    let _ = Unique.parse_u16_unique (B32.reveal input) in
+    let _ = Unique.parse_u16_unique e (B32.reveal input) in
     [@inline_let]
-    let res : option (U16.t * U32.t) = Aux.parse32_u16 input in
-    (res <: (res: option (U16.t * U32.t) { parser32_correct parse_u16 input res } ))
+    let res : result (U16.t * U32.t) err = Aux.parse32_u16 e input in
+    (res <: (res: result (U16.t * U32.t) err { parser32_correct (parse_u16 e) input res } ))
   )
 
-let serialize32_u16
-: serializer32 serialize_u16
-= (fun (input: U16.t) ->
+let serialize32_u16 #err e =
+  (fun (input: U16.t) ->
     [@inline_let]
-    let _ = Unique.serialize_u16_unique input in
+    let _ = Unique.serialize_u16_unique e input in
     [@inline_let]
-    let res : bytes32 = Aux.serialize32_u16 input in
-    (res <: (res: bytes32 { serializer32_correct #_ #_ #parse_u16 serialize_u16 input res } )))
+    let res : bytes32 = Aux.serialize32_u16 e input in
+    (res <: (res: bytes32 { serializer32_correct (serialize_u16 e) input res } )))
 
-let parse32_u32 =
+let parse32_u32 #err e =
   (fun input ->
     [@inline_let]
-    let _ = Unique.parse_u32_unique (B32.reveal input) in
+    let _ = Unique.parse_u32_unique e (B32.reveal input) in
     [@inline_let]
-    let res : option (U32.t * U32.t) = Aux.parse32_u32 input in
-    (res <: (res: option (U32.t * U32.t) { parser32_correct parse_u32 input res } ))
+    let res : result (U32.t * U32.t) err = Aux.parse32_u32 e input in
+    (res <: (res: result (U32.t * U32.t) err { parser32_correct (parse_u32 e) input res } ))
   )
 
-let serialize32_u32
-: serializer32 serialize_u32
-= (fun (input: U32.t) ->
+let serialize32_u32 #err e =
+  (fun (input: U32.t) ->
     [@inline_let]
-    let _ = Unique.serialize_u32_unique input in
+    let _ = Unique.serialize_u32_unique e input in
     [@inline_let]
-    let res : bytes32 = Aux.serialize32_u32 input in
-    (res <: (res: bytes32 { serializer32_correct #_ #_ #parse_u32 serialize_u32 input res } )))
+    let res : bytes32 = Aux.serialize32_u32 e input in
+    (res <: (res: bytes32 { serializer32_correct (serialize_u32 e) input res } )))
