src/lowparse/LowParse.SLow.List.fst
@@ -13,23 +13,22 @@ module L = FStar.List.Tot
 let rec parse_list_tailrec'
   (#k: parser_kind)
   (#t: Type0)
-  (#p: parser k t)
+  (#err: Type0)
+  (#p: parser k t err)
   (p32: parser32 p)
+  (u: unit { k.parser_kind_low > 0 } )
   (b: bytes32)
   (aux: list t)
-: GTot (option (list t))
+: GTot (result (list t) err)
   (decreases (B32.length b))
 = if B32.len b = 0ul
   then 
-    Some (L.rev aux)
+    Correct (L.rev aux)
   else
     match p32 b with
-    | None -> None
-    | Some (v, n) ->
-      if n = 0ul
-      then None (* elements cannot be empty *)
-      else
-	parse_list_tailrec' p32 (B32.slice b n (B32.len b)) (v :: aux)
+    | Error e -> Error e
+    | Correct (v, n) ->
+	parse_list_tailrec' p32 u (B32.slice b n (B32.len b)) (v :: aux)
 
 let list_append_rev_cons
   (#t: Type)
@@ -43,17 +42,19 @@ let list_append_rev_cons
 let rec parse_list_tailrec'_correct'
   (#k: parser_kind)
   (#t: Type0)
-  (#p: parser k t)
+  (#err: Type0)
+  (#p: parser k t err)
   (p32: parser32 p)
+  (u: unit { k.parser_kind_low > 0 } )
   (b: bytes32)
   (aux: list t)
 : Lemma
   (requires True)
   (ensures (
-    parse_list_tailrec' p32 b aux == (
-    match parse (parse_list p) (B32.reveal b) with
-    | Some (l, n) -> Some (L.append (L.rev aux) l)
-    | None -> None
+    parse_list_tailrec' p32 u b aux == (
+    match parse (parse_list p u) (B32.reveal b) with
+    | Correct (l, n) -> Correct (L.append (L.rev aux) l)
+    | Error e -> Error e
   )))
   (decreases (B32.length b))
 = if B32.len b = 0ul
@@ -61,31 +62,31 @@ let rec parse_list_tailrec'_correct'
     L.append_l_nil (L.rev aux)
   else
     match p32 b with
-    | None -> ()
-    | Some (v, n) ->
-      if n = 0ul
-      then ()
-      else begin
+    | Error e -> ()
+    | Correct (v, n) ->
+      begin
 	let s = B32.slice b n (B32.len b) in
-	parse_list_tailrec'_correct' p32 s (v :: aux);
-	match parse (parse_list p) (B32.reveal s) with
-	| Some (l, n') ->
+	parse_list_tailrec'_correct' p32 u s (v :: aux);
+	match parse (parse_list p u) (B32.reveal s) with
+	| Correct (l, n') ->
           list_append_rev_cons v aux l
-        | None -> ()
+        | Error e -> ()
       end
 
 let parse_list_tailrec'_correct
   (#k: parser_kind)
   (#t: Type0)
-  (#p: parser k t)
+  (#err: Type0)
+  (#p: parser k t err)
   (p32: parser32 p)
+  (u: unit { k.parser_kind_low > 0 } )
   (b: bytes32)
 : Lemma
-  begin match parse (parse_list p) (B32.reveal b) with
-  | Some (l, n) -> parse_list_tailrec' p32 b [] == Some l
-  | None -> parse_list_tailrec' p32 b [] == None
+  begin match parse (parse_list p u) (B32.reveal b) with
+  | Correct (l, n) -> parse_list_tailrec' p32 u b [] == Correct l
+  | Error e -> parse_list_tailrec' p32 u b [] == Error e
   end
-= parse_list_tailrec'_correct' p32 b []
+= parse_list_tailrec'_correct' p32 u b []
 
 let list_rev_inv
   (#t: Type)
@@ -120,106 +121,114 @@ let list_rev
 let parse_list_tailrec_inv
   (#k: parser_kind)
   (#t: Type0)
-  (#p: parser k t)
+  (#err: Type0)
+  (#p: parser k t err)
   (p32: parser32 p)
+  (u: unit { k.parser_kind_low > 0 } )
   (input: bytes32)
   (b: bool)
-  (x: option (bytes32 * list t))
+  (x: result (bytes32 * list t) err)
 : GTot Type0
 = match x with
-  | Some (input', accu') ->
-    parse_list_tailrec' p32 input [] == parse_list_tailrec' p32 input' accu' /\
+  | Correct (input', accu') ->
+    parse_list_tailrec' p32 u input [] == parse_list_tailrec' p32 u input' accu' /\
     (b == false ==> B32.length input' == 0)
-  | None -> 
-    b == false /\ None? (parse_list_tailrec' p32 input [])
+  | Error e -> 
+    b == false /\ parse_list_tailrec' p32 u input [] == Error e
 
 let parse_list_tailrec_measure
   (#t: Type0)
-  (x: option (bytes32 * list t))
+  (#err: Type0)
+  (x: result (bytes32 * list t) err)
 : GTot nat
 = match x with
-  | None -> 0
-  | Some (input', _) -> B32.length input'
+  | Error _ -> 0
+  | Correct (input', _) -> B32.length input'
 
 inline_for_extraction
 let parse_list_tailrec_body
   (#k: parser_kind)
   (#t: Type0)
-  (#p: parser k t)
+  (#err: Type0)
+  (#p: parser k t err)
   (p32: parser32 p)
+  (u: unit { k.parser_kind_low > 0 } )
   (input: bytes32)
-: (x: option (bytes32 * list t)) ->
-  Pure (bool * option (bytes32 * list t))
-  (requires (parse_list_tailrec_inv p32 input true x))
+: (x: result (bytes32 * list t) err) ->
+  Pure (bool * result (bytes32 * list t) err)
+  (requires (parse_list_tailrec_inv p32 u input true x))
   (ensures (fun (continue, y) ->
-    parse_list_tailrec_inv p32 input continue y /\
+    parse_list_tailrec_inv p32 u input continue y /\
     (if continue then parse_list_tailrec_measure y < parse_list_tailrec_measure x else True)
   ))
-= fun (x: option (bytes32 * list t)) ->
-  let (Some (input', accu')) = x in
+= fun (x: result (bytes32 * list t) err) ->
+  let (Correct (input', accu')) = x in
   let len = B32.len input' in
   if len = 0ul
   then (false, x)
   else
     match p32 input' with
-    | Some (v, consumed) ->
-      if consumed = 0ul
-      then (false, None)
-      else
+    | Correct (v, consumed) ->
         let input'' = B32.slice input' consumed len in
-        (true, Some (input'', v :: accu'))
-    | None -> (false, None)
+        (true, Correct (input'', v :: accu'))
+    | Error e -> (false, Error e)
 
 inline_for_extraction
 let parse_list_tailrec
   (#k: parser_kind)
   (#t: Type0)
-  (#p: parser k t)
+  (#err: Type0)
+  (#p: parser k t err)
   (p32: parser32 p)
+  (u: unit { k.parser_kind_low > 0 } )
   (input: bytes32)
-: Tot (res: option (list t) { res == parse_list_tailrec' p32 input [] } )
+: Tot (res: result (list t) err { res == parse_list_tailrec' p32 u input [] } )
 = let accu =
     CL.total_while
-      (parse_list_tailrec_measure #t)
-      (parse_list_tailrec_inv p32 input)
-      (fun x -> parse_list_tailrec_body p32 input x)
-      (Some (input, []))
+      (parse_list_tailrec_measure #t #err)
+      (parse_list_tailrec_inv p32 u input)
+      (fun x -> parse_list_tailrec_body p32 u input x)
+      (Correct (input, []))
   in
   match accu with
-  | None -> None
-  | Some (_, accu') -> Some (list_rev accu')
+  | Error e -> Error e
+  | Correct (_, accu') -> Correct (list_rev accu')
 
 inline_for_extraction
 let parse32_list
   (#k: parser_kind)
   (#t: Type0)
-  (#p: parser k t)
+  (#err: Type0)
+  (#p: parser k t err)
   (p32: parser32 p)
-: Tot (parser32 (parse_list p))
+  (u: unit { k.parser_kind_low > 0 } )
+: Tot (parser32 (parse_list p u))
 = fun (input: bytes32) -> ((
-    parse_list_tailrec'_correct p32 input;
-    match parse_list_tailrec p32 input with
-    | None -> None
-    | Some res ->
-      parse_list_bare_consumed p (B32.reveal input);
-      Some (res, B32.len input)
-  ) <: (res: option (list t * U32.t) { parser32_correct (parse_list p) input res } ))
+    parse_list_tailrec'_correct p32 u input;
+    match parse_list_tailrec p32 u input with
+    | Error e -> Error e
+    | Correct res ->
+      parse_list_bare_consumed p u (B32.reveal input);
+      Correct (res, B32.len input)
+  ) <: (res: result (list t * U32.t) err { parser32_correct (parse_list p u) input res } ))
 
 let rec partial_serialize32_list'
-  (#t: Type0)
   (#k: parser_kind)
-  (p: parser k t)
-  (s: serializer p)
+  (#t: Type0)
+  (#err: Type0)
+  (#p: parser k t err)
+  (#s: serializer p)
   (s32: partial_serializer32 s)
+  (u: unit { k.parser_kind_low > 0 } )
   (input: list t)
 : Ghost bytes32
   (requires (
     serialize_list_precond k /\ (
-    Seq.length (serialize (serialize_list p s) input) < 4294967296
+    Seq.length (serialize (serialize_list s u) input) < 4294967296
   )))
   (ensures (fun (res: bytes32) ->
     serialize_list_precond k /\
-    serializer32_correct (serialize_list p s) input res
+    serializer32_correct (serialize_list s u) input res
   ))
   (decreases input)
 = match input with
@@ -228,29 +237,31 @@ let rec partial_serialize32_list'
     assert (Seq.equal (B32.reveal res) (Seq.createEmpty));
     res
   | a :: q ->
-    serialize_list_cons p s a q;
+    serialize_list_cons s u a q;
     let sa = s32 a in
-    let sq = partial_serialize32_list' p s s32 q in
+    let sq = partial_serialize32_list' s32 u q in
     let res = B32.append sa sq in
     res
 
 let rec partial_serialize32_list_tailrec'
-  (#t: Type0)
   (#k: parser_kind)
-  (p: parser k t)
-  (s: serializer p)
+  (#t: Type0)
+  (#err: Type0)
+  (#p: parser k t err)
+  (#s: serializer p)
   (s32: partial_serializer32 s)
+  (u: unit { k.parser_kind_low > 0 } )
   (accu: bytes32)
   (input: list t)
 : Ghost bytes32
   (requires (
     serialize_list_precond k /\ (
-    B32.length accu + Seq.length (serialize (serialize_list p s) input) < 4294967296
+    B32.length accu + Seq.length (serialize (serialize_list s u) input) < 4294967296
   )))
   (ensures (fun (res: bytes32) ->
     serialize_list_precond k /\
-    Seq.length (serialize (serialize_list p s) input) < 4294967296 /\
-    B32.reveal res == Seq.append (B32.reveal accu) (B32.reveal (partial_serialize32_list' p s s32 input))
+    Seq.length (serialize (serialize_list s u) input) < 4294967296 /\
+    B32.reveal res == Seq.append (B32.reveal accu) (B32.reveal (partial_serialize32_list' s32 u input))
   ))
   (decreases input)
 = match input with
@@ -258,30 +269,32 @@ let rec partial_serialize32_list_tailrec'
     Seq.append_empty_r (B32.reveal accu);
     accu
   | a :: q ->
-    serialize_list_cons p s a q;
+    serialize_list_cons s u a q;
     let sa = s32 a in
     let accu' = B32.append accu sa in
-    Seq.append_assoc (B32.reveal accu) (B32.reveal sa) (B32.reveal (partial_serialize32_list' p s s32 q));
-    partial_serialize32_list_tailrec' p s s32 accu' q
+    Seq.append_assoc (B32.reveal accu) (B32.reveal sa) (B32.reveal (partial_serialize32_list' s32 u q));
+    partial_serialize32_list_tailrec' s32 u accu' q
 
 let partial_serialize32_list'_inv
-  (#t: Type0)
   (#k: parser_kind)
-  (p: parser k t)
-  (s: serializer p)
+  (#t: Type0)
+  (#err: Type0)
+  (#p: parser k t err)
+  (#s: serializer p)
   (s32: partial_serializer32 s)
+  (u: unit { k.parser_kind_low > 0 } )
   (input: list t)
   (continue: bool)
   (x: bytes32 * list t)
 : GTot Type0
 = serialize_list_precond k /\
-  Seq.length (serialize (serialize_list p s) input) < 4294967296 /\ (
+  Seq.length (serialize (serialize_list s u) input) < 4294967296 /\ (
     let (accu, input') = x in
-    B32.length accu + Seq.length (serialize (serialize_list p s) input') < 4294967296 /\
+    B32.length accu + Seq.length (serialize (serialize_list s u) input') < 4294967296 /\
     serializer32_correct
-      (serialize_list p s)
+      (serialize_list s u)
       input
-      (partial_serialize32_list_tailrec' p s s32 accu input') /\
+      (partial_serialize32_list_tailrec' s32 u accu input') /\
     (continue == false ==> L.length input' == 0)
   )
 
@@ -293,17 +306,19 @@ let partial_serialize32_list'_measure
 
 inline_for_extraction
 let partial_serialize32_list'_body
-  (#t: Type0)
   (#k: parser_kind)
-  (p: parser k t)
-  (s: serializer p)
+  (#t: Type0)
+  (#err: Type0)
+  (#p: parser k t err)
+  (#s: serializer p)
   (s32: partial_serializer32 s)
+  (u: unit { k.parser_kind_low > 0 } )
   (input: list t)
 : (x: (bytes32 * list t)) ->
   Pure (bool * (bytes32 * list t))
-  (requires (partial_serialize32_list'_inv p s s32 input true x))
+  (requires (partial_serialize32_list'_inv s32 u input true x))
   (ensures (fun (continue, y) ->
-    partial_serialize32_list'_inv p s s32 input continue y /\
+    partial_serialize32_list'_inv s32 u input continue y /\
     (continue == true ==> partial_serialize32_list'_measure y < partial_serialize32_list'_measure x)
   ))
 = fun (x: bytes32 * list t) ->
@@ -316,54 +331,57 @@ let partial_serialize32_list'_body
     (true, (accu', q))
 
 let partial_serialize32_list'_init
-  (#t: Type0)
   (#k: parser_kind)
-  (p: parser k t)
-  (s: serializer p)
+  (#t: Type0)
+  (#err: Type0)
+  (#p: parser k t err)
+  (#s: serializer p)
   (s32: partial_serializer32 s)
+  (u: unit { k.parser_kind_low > 0 } )
   (input: list t)
 : Lemma
   (requires (
     serialize_list_precond k /\
-    Seq.length (serialize (serialize_list p s) input) < 4294967296
+    Seq.length (serialize (serialize_list s u) input) < 4294967296
   ))
   (ensures (
-    partial_serialize32_list'_inv p s s32 input true (B32.empty_bytes, input)
+    partial_serialize32_list'_inv s32 u input true (B32.empty_bytes, input)
   ))
 = assert (Seq.equal (B32.reveal B32.empty_bytes) Seq.createEmpty);
-  Seq.append_empty_l (B32.reveal (partial_serialize32_list' p s s32 input));
-  assert (B32.reveal (partial_serialize32_list' p s s32 input) == B32.reveal (partial_serialize32_list_tailrec' p s s32 B32.empty_bytes input));
-  assert (serializer32_correct (serialize_list p s) input (partial_serialize32_list_tailrec' p s s32 B32.empty_bytes input))
+  Seq.append_empty_l (B32.reveal (partial_serialize32_list' s32 u input));
+  assert (B32.reveal (partial_serialize32_list' s32 u input) == B32.reveal (partial_serialize32_list_tailrec' s32 u B32.empty_bytes input));
+  assert (serializer32_correct (serialize_list s u) input (partial_serialize32_list_tailrec' s32 u B32.empty_bytes input))
 
 inline_for_extraction
 let partial_serialize32_list
-  (#t: Type0)
   (#k: parser_kind)
-  (p: parser k t)
-  (s: serializer p)
+  (#t: Type0)
+  (#err: Type0)
+  (#p: parser k t err)
+  (#s: serializer p)
   (s32: partial_serializer32 s)
   (u: unit {
     serialize_list_precond k
   })
-: Tot (partial_serializer32 (serialize_list p s))
-= fun (input: list t { Seq.length (serialize (serialize_list p s) input) < 4294967296 } ) -> ((
+: Tot (partial_serializer32 (serialize_list s ()))
+= fun (input: list t { Seq.length (serialize (serialize_list s ()) input) < 4294967296 } ) -> ((
     let (res, _) =
-      partial_serialize32_list'_init p s s32 input;
+      partial_serialize32_list'_init s32 () input;
       CL.total_while
         partial_serialize32_list'_measure
-        (partial_serialize32_list'_inv p s s32 input)
-        (fun x -> partial_serialize32_list'_body p s s32 input x)
+        (partial_serialize32_list'_inv s32 () input)
+        (fun x -> partial_serialize32_list'_body s32 () input x)
         (B32.empty_bytes, input)
     in
     res
-  ) <: (res: bytes32 { serializer32_correct (serialize_list p s) input res }))
+  ) <: (res: bytes32 { serializer32_correct (serialize_list s ()) input res }))
 
 let size32_list_inv
-  (#t: Type0)
   (#k: parser_kind)
-  (#p: parser k t)
-  (#s: serializer p)
-  (s32: size32 s)
+  (#t: Type0)
+  (#err: Type0)
+  (#p: parser k t err)
+  (s: serializer p)
   (u: unit {
     serialize_list_precond k
   })
@@ -372,13 +390,13 @@ let size32_list_inv
   (accu: (U32.t * list t))
 : GTot Type0
 = let (len, rem) = accu in
-  let sz = Seq.length (serialize (serialize_list p s) input) in
+  let sz = Seq.length (serialize (serialize_list s ()) input) in
   if continue
   then
     U32.v len < U32.v u32_max /\
-    sz == U32.v len + Seq.length (serialize (serialize_list p s) rem)
+    sz == U32.v len + Seq.length (serialize (serialize_list s ()) rem)
   else
-    size32_postcond (serialize_list p s) input len
+    size32_postcond (serialize_list s ()) input len
 
 let size32_list_measure
   (#t: Type0)
@@ -389,9 +407,10 @@ let size32_list_measure
 
 inline_for_extraction
 let size32_list_body
-  (#t: Type0)
   (#k: parser_kind)
-  (#p: parser k t)
+  (#t: Type0)
+  (#err: Type0)
+  (#p: parser k t err)
   (#s: serializer p)
   (s32: size32 s)
   (u: unit {
@@ -400,9 +419,9 @@ let size32_list_body
   (input: list t)
 : (x: (U32.t * list t)) ->
   Pure (bool * (U32.t * list t))
-  (requires (size32_list_inv s32 u input true x))
+  (requires (size32_list_inv s u input true x))
   (ensures (fun (continue, y) ->
-    size32_list_inv s32 u input continue y /\
+    size32_list_inv s u input continue y /\
     (continue == true ==> size32_list_measure y < size32_list_measure x)
   ))
 = fun accu ->
@@ -418,22 +437,23 @@ let size32_list_body
 
 inline_for_extraction
 let size32_list
-  (#t: Type0)
   (#k: parser_kind)
-  (#p: parser k t)
+  (#t: Type0)
+  (#err: Type0)
+  (#p: parser k t err)
   (#s: serializer p)
   (s32: size32 s)
   (u: unit {
     serialize_list_precond k
   })
-: Tot (size32 (serialize_list p s))
+: Tot (size32 (serialize_list s ()))
 = fun input ->
   [@inline_let]
   let (len, _) =
     CL.total_while
       size32_list_measure
-      (size32_list_inv s32 u input)
+      (size32_list_inv s u input)
       (fun x -> size32_list_body s32 u input x)
       (0ul, input)
   in
-  (len <: (len : U32.t { size32_postcond (serialize_list p s) input len } ))
+  (len <: (len : U32.t { size32_postcond (serialize_list s ()) input len } ))
