src/lowparse/LowParse.SLow.VLData.fst
@@ -9,45 +9,55 @@ module B32 = LowParse.Bytes32
 
 inline_for_extraction
 let serialize32_bounded_integer_1
-: (serializer32 (serialize_bounded_integer 1))
+  (#err: Type0)
+  (e: err)
+: Tot (serializer32 (serialize_bounded_integer 1 e))
 = (fun (input: bounded_integer 1) ->
     let b = E.n_to_be_1 _ _ (E.u32 ()) input in
-    (b <: (res: B32.bytes { serializer32_correct (serialize_bounded_integer 1) input res } ))
+    (b <: (res: B32.bytes { serializer32_correct (serialize_bounded_integer 1 e) input res } ))
   )
 
 inline_for_extraction
 let serialize32_bounded_integer_2
-: (serializer32 (serialize_bounded_integer 2))
+  (#err: Type0)
+  (e: err)
+: Tot (serializer32 (serialize_bounded_integer 2 e))
 = (fun (input: bounded_integer 2) ->
     let b = E.n_to_be_2 _ _ (E.u32 ()) input in
-    (b <: (res: B32.bytes { serializer32_correct (serialize_bounded_integer 2) input res } ))
+    (b <: (res: B32.bytes { serializer32_correct (serialize_bounded_integer 2 e) input res } ))
   )
 
 inline_for_extraction
 let serialize32_bounded_integer_3
-: (serializer32 (serialize_bounded_integer 3))
+  (#err: Type0)
+  (e: err)
+: Tot (serializer32 (serialize_bounded_integer 3 e))
 = (fun (input: bounded_integer 3) ->
     let b = E.n_to_be_3 _ _ (E.u32 ()) input in
-    (b <: (res: B32.bytes { serializer32_correct (serialize_bounded_integer 3) input res } ))
+    (b <: (res: B32.bytes { serializer32_correct (serialize_bounded_integer 3 e) input res } ))
   )
 
 inline_for_extraction
 let serialize32_bounded_integer_4
-: (serializer32 (serialize_bounded_integer 4))
+  (#err: Type0)
+  (e: err)
+: Tot (serializer32 (serialize_bounded_integer 4 e))
 = (fun (input: bounded_integer 4) ->
     let b = E.n_to_be_4 _ _ (E.u32 ()) input in
-    (b <: (res: B32.bytes { serializer32_correct (serialize_bounded_integer 4) input res } ))
+    (b <: (res: B32.bytes { serializer32_correct (serialize_bounded_integer 4 e) input res } ))
   )
 
 inline_for_extraction
 let serialize32_bounded_integer
+  (#err: Type0)
   (sz: integer_size)
-: Tot (serializer32 (serialize_bounded_integer sz))
+  (e: err)
+: Tot (serializer32 (serialize_bounded_integer sz e))
 = match sz with
-  | 1 -> serialize32_bounded_integer_1
-  | 2 -> serialize32_bounded_integer_2
-  | 3 -> serialize32_bounded_integer_3
-  | 4 -> serialize32_bounded_integer_4
+  | 1 -> serialize32_bounded_integer_1 e
+  | 2 -> serialize32_bounded_integer_2 e
+  | 3 -> serialize32_bounded_integer_3 e
+  | 4 -> serialize32_bounded_integer_4 e
 
 inline_for_extraction
 let decode32_bounded_integer_1
@@ -94,11 +104,16 @@ let decode32_bounded_integer
   | 4 -> decode32_bounded_integer_4
 
 inline_for_extraction
-let parse32_bounded_integer (sz: integer_size) : Tot (parser32 (parse_bounded_integer sz)) =
-  [@inline_let]
+let parse32_bounded_integer
+  (#err: Type0)
+  (sz: integer_size)
+  (e: err)
+: Tot (parser32 (parse_bounded_integer sz e))
+= [@inline_let]
   let _ = decode_bounded_integer_injective sz in
   make_total_constant_size_parser32 sz (U32.uint_to_t sz)
     (decode_bounded_integer sz)
+    e
     ()
     (decode32_bounded_integer sz)
 
@@ -110,11 +125,13 @@ let parse32_vldata_payload
   (f: (bounded_integer sz -> GTot bool))
   (#k: parser_kind)
   (#t: Type0)
-  (#p: parser k t)
+  (#err: Type0)
+  (#p: parser k t err)
   (p32: parser32 p)
+  (e: err)
   (i: bounded_integer sz { f i == true } )
-: Tot (parser32 (parse_vldata_payload sz f p i))
-= fun (input: bytes32) -> parse32_fldata p32 (U32.v i) i input
+: Tot (parser32 (parse_vldata_payload sz f p e i))
+= fun (input: bytes32) -> parse32_fldata p32 (U32.v i) i e input
 
 inline_for_extraction
 let parse32_vldata_gen
@@ -123,28 +140,35 @@ let parse32_vldata_gen
   (f' : (x: bounded_integer sz) -> Tot (y: bool {y == f x}))
   (#k: parser_kind)
   (#t: Type0)
-  (#p: parser k t)
+  (#err: Type0)
+  (#p: parser k t err)
   (p32: parser32 p)
-: Tot (parser32 (parse_vldata_gen sz f p))
+  (e_size_incomplete: err)
+  (e_size_invalid: err)
+  (e_payload: err)
+: Tot (parser32 (parse_vldata_gen sz f p e_size_incomplete e_size_invalid e_payload))
 = [@inline_let]
-  let _ = parse_fldata_and_then_cases_injective sz f p in
+  let _ = parse_fldata_and_then_cases_injective sz f p e_payload in
   [@inline_let]
   let _ = parse_vldata_gen_kind_correct sz in
   parse32_and_then
-    (parse32_filter (parse32_bounded_integer sz) f f')
-    (parse_vldata_payload sz f p)
+    (parse32_filter (parse32_bounded_integer sz e_size_incomplete) f e_size_invalid f')
+    (parse_vldata_payload sz f p e_payload)
     ()
-    (parse32_vldata_payload sz f p32)
+    (parse32_vldata_payload sz f p32 e_payload)
 
 inline_for_extraction
 let parse32_vldata
   (sz: integer_size)
   (#k: parser_kind)
   (#t: Type0)
-  (#p: parser k t)
+  (#err: Type0)
+  (#p: parser k t err)
   (p32: parser32 p)
-: Tot (parser32 (parse_vldata sz p))
-= parse32_vldata_gen sz (unconstrained_bounded_integer sz) (fun _ -> true) p32
+  (e_size: err)
+  (e_payload: err)
+: Tot (parser32 (parse_vldata sz p e_size e_payload))
+= parse32_vldata_gen sz (unconstrained_bounded_integer sz) (fun _ -> true) p32 e_size e_size e_payload
 
 #set-options "--z3rlimit 32"
 
@@ -156,14 +180,16 @@ let parse32_bounded_vldata
   (max32: U32.t { U32.v max32 == max } )
   (#k: parser_kind)
   (#t: Type0)
-  (#p: parser k t)
+  (#err: Type0)
+  (#p: parser k t err)
   (p32: parser32 p)
-: Tot (parser32 (parse_bounded_vldata min max p))
+  (e_size_incomplete e_size_invalid e_payload: err)
+: Tot (parser32 (parse_bounded_vldata min max p e_size_incomplete e_size_invalid e_payload))
 = [@inline_let]
   let _ = parse_bounded_vldata_correct min max p in
   [@inline_let]
   let sz : integer_size = (log256' max) in
-  (fun input -> parse32_vldata_gen sz (in_bounds min max) (fun i -> not (U32.lt i min32 || U32.lt max32 i)) p32 input)
+  (fun input -> parse32_vldata_gen sz (in_bounds min max) (fun i -> not (U32.lt i min32 || U32.lt max32 i)) p32 e_size_incomplete e_size_invalid e_payload input)
 
 inline_for_extraction
 let parse32_bounded_vldata_strong'
@@ -173,26 +199,25 @@ let parse32_bounded_vldata_strong'
   (max32: U32.t { U32.v max32 == max } )
   (#k: parser_kind)
   (#t: Type0)
-  (#p: parser k t)
+  (#err: Type0)
+  (#p: parser k t err)
   (s: serializer p)
   (p32: parser32 p)
+  (e_size_incomplete e_size_invalid e_payload: err)
   (input: bytes32)
-: Tot (option (parse_bounded_vldata_strong_t min max #k #t #p s * U32.t))
+: Tot (result (parse_bounded_vldata_strong_t min max s * U32.t) err)
 = let res =
     parse32_strengthen
-      #(parse_bounded_vldata_kind min max)
-      #t
-      #(parse_bounded_vldata min max #k #t p)
-      (parse32_bounded_vldata min min32 max max32 #k #t #p p32)
-      (parse_bounded_vldata_strong_pred min max #k #t #p s)
-      (parse_bounded_vldata_strong_correct min max #k #t #p s)
+      (parse32_bounded_vldata min min32 max max32 p32 e_size_incomplete e_size_invalid e_payload)
+      (parse_bounded_vldata_strong_pred min max s)
+      (parse_bounded_vldata_strong_correct min max s e_size_incomplete e_size_invalid e_payload)
       input
   in
   match res with
-  | None -> None
-  | Some (x, consumed) ->
+  | Error e -> Error e
+  | Correct (x, consumed) ->
     let x1 : t = x in
-    Some ((x1 <: parse_bounded_vldata_strong_t min max #k #t #p s), consumed)
+    Correct ((x1 <: parse_bounded_vldata_strong_t min max s), consumed)
 
 let parse32_bounded_vldata_strong_correct
   (min: nat)
@@ -201,31 +226,30 @@ let parse32_bounded_vldata_strong_correct
   (max32: U32.t { U32.v max32 == max } )
   (#k: parser_kind)
   (#t: Type0)
-  (#p: parser k t)
+  (#err: Type0)
+  (#p: parser k t err)
   (s: serializer p)
   (p32: parser32 p)
+  (e_size_incomplete e_size_invalid e_payload: err)
   (input: bytes32)
 : Lemma
-  ( let res : option (parse_bounded_vldata_strong_t min max s * U32.t) = 
-      parse32_bounded_vldata_strong' min min32 max max32 s p32 input
+  ( let res : result (parse_bounded_vldata_strong_t min max s * U32.t) err = 
+      parse32_bounded_vldata_strong' min min32 max max32 s p32 e_size_incomplete e_size_invalid e_payload input
     in
-    parser32_correct (parse_bounded_vldata_strong min max s) input res)
+    parser32_correct (parse_bounded_vldata_strong min max s e_size_incomplete e_size_invalid e_payload) input res)
 = let res =
     parse32_strengthen
-      #(parse_bounded_vldata_kind min max)
-      #t
-      #(parse_bounded_vldata min max #k #t p)
-      (parse32_bounded_vldata min min32 max max32 #k #t #p p32)
-      (parse_bounded_vldata_strong_pred min max #k #t #p s)
-      (parse_bounded_vldata_strong_correct min max #k #t #p s)
+      (parse32_bounded_vldata min min32 max max32 p32 e_size_incomplete e_size_invalid e_payload)
+      (parse_bounded_vldata_strong_pred min max s)
+      (parse_bounded_vldata_strong_correct min max s e_size_incomplete e_size_invalid e_payload)
       input
   in
   match res with
-  | None -> ()
-  | Some (x, consumed) ->
+  | Error _ -> ()
+  | Correct (x, consumed) ->
     let x1 : t = x in
-    let res = Some ((x1 <: parse_bounded_vldata_strong_t min max #k #t #p s), consumed) in
-    assert (parser32_correct (parse_bounded_vldata_strong min max s) input res)
+    let res = Correct ((x1 <: parse_bounded_vldata_strong_t min max s), consumed) in
+    assert (parser32_correct (parse_bounded_vldata_strong min max s e_size_incomplete e_size_invalid e_payload) input res)
 
 inline_for_extraction
 let parse32_bounded_vldata_strong
@@ -235,15 +259,17 @@ let parse32_bounded_vldata_strong
   (max32: U32.t { U32.v max32 == max } )
   (#k: parser_kind)
   (#t: Type0)
-  (#p: parser k t)
+  (#err: Type0)
+  (#p: parser k t err)
   (s: serializer p)
   (p32: parser32 p)
-: Tot (parser32 #(parse_bounded_vldata_kind min max) #(parse_bounded_vldata_strong_t min max s) (parse_bounded_vldata_strong min max s))
+  (e_size_incomplete e_size_invalid e_payload: err)
+: Tot (parser32 (parse_bounded_vldata_strong min max s e_size_incomplete e_size_invalid e_payload))
 = make_parser32
-    (parse_bounded_vldata_strong min max s)
+    (parse_bounded_vldata_strong min max s e_size_incomplete e_size_invalid e_payload)
     (fun input ->
-       parse32_bounded_vldata_strong_correct min min32 max max32 s p32 input;
-       parse32_bounded_vldata_strong' min min32 max max32 s p32 input
+       parse32_bounded_vldata_strong_correct min min32 max max32 s p32 e_size_incomplete e_size_invalid e_payload input;
+       parse32_bounded_vldata_strong' min min32 max max32 s p32 e_size_incomplete e_size_invalid e_payload input
     )
 
 inline_for_extraction
@@ -252,14 +278,16 @@ let serialize32_bounded_vldata_strong'
   (max: nat { min <= max /\ max > 0 /\ max < 4294967292 } ) // NOTE here: max must be less than 2^32 - 4
   (#k: parser_kind)
   (#t: Type0)
-  (#p: parser k t)
+  (#err: Type0)
+  (#p: parser k t err)
   (#s: serializer p)
   (s32: partial_serializer32 s)
+  (e_size_incomplete: err)
 : Tot (parse_bounded_vldata_strong_t min max s -> Tot bytes32)
 = [@inline_let]
   let sz : integer_size = log256' max in
   [@inline_let]
-  let ser : serializer32 (serialize_bounded_integer sz) = serialize32_bounded_integer sz in
+  let ser : serializer32 (serialize_bounded_integer sz e_size_incomplete) = serialize32_bounded_integer sz e_size_incomplete in
   (fun (input: parse_bounded_vldata_strong_t min max s) ->
     let pl = s32 input in
     let len = B32.len pl in
@@ -275,27 +303,29 @@ let serialize32_bounded_vldata_strong_correct
   (max: nat { min <= max /\ max > 0 /\ max < 4294967292 } ) // NOTE here: max must be less than 2^32 - 4
   (#k: parser_kind)
   (#t: Type0)
-  (#p: parser k t)
+  (#err: Type0)
+  (#p: parser k t err)
   (#s: serializer p)
   (s32: partial_serializer32 s)
+  (e_size_incomplete e_size_invalid e_payload: err)
   (input: parse_bounded_vldata_strong_t min max s)
 : Lemma
-  (serializer32_correct (serialize_bounded_vldata_strong min max s) input (serialize32_bounded_vldata_strong' min max s32 input))
+  (serializer32_correct (serialize_bounded_vldata_strong min max s e_size_incomplete e_size_invalid e_payload) input (serialize32_bounded_vldata_strong' min max s32 e_size_incomplete input))
 = let sz : integer_size = log256' max in
-  let ser : serializer32 (serialize_bounded_integer sz) = serialize32_bounded_integer sz in
+  let ser : serializer32 (serialize_bounded_integer sz e_size_incomplete) = serialize32_bounded_integer sz e_size_incomplete in
   let pl = s32 input in
   assert (B32.reveal pl == s input);
   let len = B32.len pl in
   let nlen = U32.v len in
   assert (min <= nlen /\ nlen <= max);
   let slen = ser (len <: bounded_integer sz) in
-  assert (B32.reveal slen == serialize (serialize_bounded_integer sz) len);
+  assert (B32.reveal slen == serialize (serialize_bounded_integer sz e_size_incomplete) len);
   seq_slice_append_l (B32.reveal slen) (B32.reveal pl);
   seq_slice_append_r (B32.reveal slen) (B32.reveal pl);
   let res : bytes32 = B32.b32append slen pl in
   assert (B32.reveal res == Seq.append (B32.reveal slen) (B32.reveal pl));
-  assert (B32.reveal res == serialize_bounded_vldata_strong' min max s input);
-  assert (serializer32_correct (serialize_bounded_vldata_strong min max s) input res)
+  assert (B32.reveal res == serialize_bounded_vldata_strong' min max s e_size_incomplete input);
+  assert (serializer32_correct (serialize_bounded_vldata_strong min max s e_size_incomplete e_size_invalid e_payload) input res)
 
 inline_for_extraction
 let serialize32_bounded_vldata_strong
@@ -303,13 +333,15 @@ let serialize32_bounded_vldata_strong
   (max: nat { min <= max /\ max > 0 /\ max < 4294967292 } ) // NOTE here: max must be less than 2^32 - 4
   (#k: parser_kind)
   (#t: Type0)
-  (#p: parser k t)
+  (#err: Type0)
+  (#p: parser k t err)
   (#s: serializer p)
   (s32: partial_serializer32 s)
-: Tot (serializer32 (serialize_bounded_vldata_strong min max s))
+  (e_size_incomplete e_size_invalid e_payload: err)
+: Tot (serializer32 (serialize_bounded_vldata_strong min max s e_size_incomplete e_size_invalid e_payload))
 = fun (input: parse_bounded_vldata_strong_t min max s) ->
-  serialize32_bounded_vldata_strong_correct min max s32 input;
-  (serialize32_bounded_vldata_strong' min max s32 input <: (res: bytes32 { serializer32_correct (serialize_bounded_vldata_strong min max s) input res } ))
+  serialize32_bounded_vldata_strong_correct min max s32 e_size_incomplete e_size_invalid e_payload input;
+  (serialize32_bounded_vldata_strong' min max s32 e_size_incomplete input <: (res: bytes32 { serializer32_correct (serialize_bounded_vldata_strong min max s e_size_incomplete e_size_invalid e_payload) input res } ))
 
 #reset-options "--z3rlimit 32 --z3cliopt smt.arith.nl=false"
 
@@ -321,7 +353,8 @@ let check_vldata_payload_size32
   (max32: U32.t { U32.v max32 == max } )
   (#k: parser_kind)
   (#t: Type0)
-  (#p: parser k t)
+  (#err: Type0)
+  (#p: parser k t err)
   (#s: serializer p)
   (s32: size32 s)
   (input: t)
@@ -356,11 +389,13 @@ let size32_bounded_vldata_strong
   (max: nat { min <= max /\ max > 0 /\ max < 4294967292 } ) // NOTE here: max must be less than 2^32 - 4, otherwise add overflows
   (#k: parser_kind)
   (#t: Type0)
-  (#p: parser k t)
+  (#err: Type0)
+  (#p: parser k t err)
   (#s: serializer p)
   (s32: size32 s)
   (sz32: U32.t { U32.v sz32 == log256' max } )
-: Tot (size32 (serialize_bounded_vldata_strong min max s))
+  (e_size_incomplete e_size_invalid e_payload: err)
+: Tot (size32 (serialize_bounded_vldata_strong min max s e_size_incomplete e_size_invalid e_payload))
 = (fun (input: parse_bounded_vldata_strong_t min max s) ->
     let len = s32 input in
     [@inline_let]
@@ -369,4 +404,4 @@ let size32_bounded_vldata_strong
     let _ = assert (min <= U32.v len /\ U32.v len <= max) in
     [@inline_let]
     let res : U32.t = U32.add sz32 len in
-    (res <: (res: U32.t { size32_postcond (serialize_bounded_vldata_strong min max s) input res  } )))
+    (res <: (res: U32.t { size32_postcond (serialize_bounded_vldata_strong min max s e_size_incomplete e_size_invalid e_payload) input res  } )))
