src/lowparse/LowParse.SLow.Array.fst
@@ -10,14 +10,16 @@ inline_for_extraction
 let parse32_array
   (#k: parser_kind)
   (#t: Type0)
-  (#p: parser k t)
+  (#err: Type0)
+  (#p: parser k t err)
   (s: serializer p)
   (p32: parser32 p)
   (array_byte_size: nat)
   (array_byte_size32: U32.t { U32.v array_byte_size32 == array_byte_size } )
   (elem_count: nat)
+  (e: err)
   (u : unit { fldata_array_precond p array_byte_size elem_count == true } )
-: Tot (parser32 (parse_array s array_byte_size elem_count))
+: Tot (parser32 (parse_array s array_byte_size elem_count e))
 = [@inline_let]
   let _ =
     fldata_to_array_inj s array_byte_size elem_count u
@@ -27,10 +29,11 @@ let parse32_array
     (fldata_to_array s array_byte_size elem_count u)
     (fun x -> fldata_to_array s array_byte_size elem_count u x)
     (parse32_fldata_strong
-      (serialize_list _ s)
-      (parse32_list p32)
+      (serialize_list s ())
+      (parse32_list p32 ())
       array_byte_size
       array_byte_size32
+      e
     )
     ()
 
@@ -38,13 +41,15 @@ inline_for_extraction
 let serialize32_array
   (#k: parser_kind)
   (#t: Type0)
-  (#p: parser k t)
+  (#err: Type0)
+  (#p: parser k t err)
   (#s: serializer p)
   (s32: partial_serializer32 s)
   (array_byte_size: nat { array_byte_size < 4294967296 } )
   (elem_count: nat)
+  (e: err)
   (u : unit { fldata_array_precond p array_byte_size elem_count == true } )
-: Tot (serializer32 (serialize_array s array_byte_size elem_count u))
+: Tot (serializer32 (serialize_array s array_byte_size elem_count e u))
 = [@inline_let]
   let _ =
     fldata_to_array_inj s array_byte_size elem_count u
@@ -58,8 +63,9 @@ let serialize32_array
     (fldata_to_array s array_byte_size elem_count u)
     _
     (serialize32_fldata_strong
-      (partial_serialize32_list _ _ s32 ())
+      (partial_serialize32_list s32 ())
       array_byte_size
+      e
     )
     (array_to_fldata s array_byte_size elem_count u)
     (fun x -> array_to_fldata s array_byte_size elem_count u x)
@@ -73,15 +79,17 @@ let parse32_vlarray
   (array_byte_size_max32: U32.t { U32.v array_byte_size_max32 == array_byte_size_max } )
   (#k: parser_kind)
   (#t: Type0)
-  (#p: parser k t)
+  (#err: Type0)
+  (#p: parser k t err)
   (s: serializer p)
   (p32: parser32 p)
   (elem_count_min: nat)
   (elem_count_max: nat)
+  (e_size_incomplete e_size_invalid e_payload: err)
   (u: unit {
     vldata_vlarray_precond array_byte_size_min array_byte_size_max p elem_count_min elem_count_max == true  
   })
-: Tot (parser32 (parse_vlarray array_byte_size_min array_byte_size_max s elem_count_min elem_count_max u))
+: Tot (parser32 (parse_vlarray array_byte_size_min array_byte_size_max s elem_count_min elem_count_max e_size_incomplete e_size_invalid e_payload u))
 = [@inline_let]
   let _ =
     vldata_to_vlarray_inj array_byte_size_min array_byte_size_max s elem_count_min elem_count_max u
@@ -95,8 +103,9 @@ let parse32_vlarray
       array_byte_size_min32
       array_byte_size_max
       array_byte_size_max32
-      (serialize_list _ s)
-      (parse32_list p32)
+      (serialize_list s ())
+      (parse32_list p32 ())
+      e_size_incomplete e_size_invalid e_payload
     )
     ()
 
@@ -106,15 +115,17 @@ let serialize32_vlarray
   (array_byte_size_max: nat { array_byte_size_max < 4294967292 } ) // NOTE here: max must be less than 2^32 - 4 to account for the size of the length header
   (#k: parser_kind)
   (#t: Type0)
-  (#p: parser k t)
+  (#err: Type0)
+  (#p: parser k t err)
   (#s: serializer p)
   (s32: partial_serializer32 s)
   (elem_count_min: nat)
   (elem_count_max: nat)
+  (e_size_incomplete e_size_invalid e_payload: err)
   (u: unit {
     vldata_vlarray_precond array_byte_size_min array_byte_size_max p elem_count_min elem_count_max == true  
   })
-: Tot (serializer32 (serialize_vlarray array_byte_size_min array_byte_size_max s elem_count_min elem_count_max u))
+: Tot (serializer32 (serialize_vlarray array_byte_size_min array_byte_size_max s elem_count_min elem_count_max e_size_incomplete e_size_invalid e_payload u))
 = [@inline_let]
   let _ =
     vldata_to_vlarray_inj array_byte_size_min array_byte_size_max s elem_count_min elem_count_max u
@@ -130,7 +141,8 @@ let serialize32_vlarray
     (serialize32_bounded_vldata_strong
       array_byte_size_min
       array_byte_size_max
-      (partial_serialize32_list _ _ s32 ())
+      (partial_serialize32_list s32 ())
+      e_size_incomplete e_size_invalid e_payload
     )
     (vlarray_to_vldata array_byte_size_min array_byte_size_max s elem_count_min elem_count_max u)
     (fun x -> vlarray_to_vldata array_byte_size_min array_byte_size_max s elem_count_min elem_count_max u x)
@@ -142,16 +154,18 @@ let size32_vlarray
   (array_byte_size_max: nat { array_byte_size_max < 4294967292 } ) // NOTE here: max must be less than 2^32 - 4 to account for the size of the length header
   (#k: parser_kind)
   (#t: Type0)
-  (#p: parser k t)
+  (#err: Type0)
+  (#p: parser k t err)
   (s: serializer p)
   (elem_count_min: nat)
   (elem_count_max: nat)
+  (e_size_incomplete e_size_invalid e_payload: err)
   (u: unit {
     vldata_vlarray_precond array_byte_size_min array_byte_size_max p elem_count_min elem_count_max == true  
   })
   (size_header_byte_size32: U32.t { U32.v size_header_byte_size32 == log256' array_byte_size_max } )
   (elem_byte_size32: U32.t { U32.v elem_byte_size32 == k.parser_kind_low } )
-: Tot (size32 (serialize_vlarray array_byte_size_min array_byte_size_max s elem_count_min elem_count_max u))
+: Tot (size32 (serialize_vlarray array_byte_size_min array_byte_size_max s elem_count_min elem_count_max e_size_incomplete e_size_invalid e_payload u))
 = [@inline_let]
   let _ =
     vldata_to_vlarray_inj array_byte_size_min array_byte_size_max s elem_count_min elem_count_max u
@@ -167,8 +181,9 @@ let size32_vlarray
     (size32_bounded_vldata_strong
       array_byte_size_min
       array_byte_size_max
-      (size32_list #_ #_ #_ #s (size32_constant s elem_byte_size32 ()) ())
+      (size32_list (size32_constant s elem_byte_size32 ()) ())
       size_header_byte_size32
+      e_size_incomplete e_size_invalid e_payload
     )
     (vlarray_to_vldata array_byte_size_min array_byte_size_max s elem_count_min elem_count_max u)
     (fun x -> vlarray_to_vldata array_byte_size_min array_byte_size_max s elem_count_min elem_count_max u x)
