src/lowparse/LowParse.Spec.Array.fst
@@ -30,18 +30,6 @@ let fldata_array_precond
   k.parser_kind_low > 0 &&
   elem_count * k.parser_kind_low = array_byte_size
 
-let parse_list_precond_of_fldata_array_precond
-  (#k: parser_kind)
-  (#t: Type0)
-  (#err: Type0)
-  (p: parser k t err)
-  (array_byte_size: nat)
-  (elem_count: nat)
-: Pure (u: unit { k.parser_kind_low > 0 } )
-  (requires (fldata_array_precond p array_byte_size elem_count == true))
-  (ensures (fun _ -> True))
-= ()
-
 let fldata_to_array_correct
   (#k: parser_kind)
   (#t: Type0)
@@ -52,16 +40,15 @@ let fldata_to_array_correct
   (elem_count: nat)
   (x: list t)
   (u1: unit { fldata_array_precond p array_byte_size elem_count == true } )
-  (u2: unit { parse_fldata_strong_pred (serialize_list _ (parse_list_precond_of_fldata_array_precond p array_byte_size elem_count) s) array_byte_size x } )
+  (u2: unit { parse_fldata_strong_pred (serialize_list s ()) array_byte_size x } )
 : Lemma
   (ensures (
     array_pred elem_count x
   ))
-= let u = (parse_list_precond_of_fldata_array_precond p array_byte_size elem_count) in
-  let y = serialize (serialize_list _ u s) x in
-  assert (parse (parse_list p u) y == Correct (x, array_byte_size));
+= let y = serialize (serialize_list s ()) x in
+  assert (parse (parse_list p ()) y == Correct (x, array_byte_size));
   assert (Seq.length y == array_byte_size);
-  list_length_constant_size_parser_correct p u y;
+  list_length_constant_size_parser_correct p () y;
   M.mul_reg_r elem_count (L.length x) k.parser_kind_low
 
 inline_for_extraction
@@ -79,7 +66,7 @@ let fldata_to_array
   (u: unit {
     fldata_array_precond p array_byte_size elem_count == true
   })
-  (x: parse_fldata_strong_t (serialize_list _ () s) array_byte_size)
+  (x: parse_fldata_strong_t (serialize_list s ()) array_byte_size)
 : Tot (array t elem_count)
 = [@inline_let]
   let (x' : list t) = x in
@@ -99,7 +86,7 @@ let fldata_to_array_inj
     fldata_array_precond p array_byte_size elem_count == true
   })
 : Lemma
-  (forall (x1 x2: parse_fldata_strong_t (serialize_list _ () s) array_byte_size) .
+  (forall (x1 x2: parse_fldata_strong_t (serialize_list s ()) array_byte_size) .
     fldata_to_array s array_byte_size elem_count u x1 == 
     fldata_to_array s array_byte_size elem_count u x2 ==>
     x1 == x2)
@@ -121,7 +108,7 @@ let parse_array
   (ensures (fun _ -> True))
 = let (u : unit { fldata_array_precond p array_byte_size elem_count == true } ) = () in
   fldata_to_array_inj s array_byte_size elem_count u;
-  parse_fldata_strong (serialize_list _ () s) array_byte_size e `parse_synth` (fldata_to_array s array_byte_size elem_count u)
+  parse_fldata_strong (serialize_list s ()) array_byte_size e `parse_synth` (fldata_to_array s array_byte_size elem_count u)
 
 let array_to_fldata_correct
   (#k: parser_kind)
@@ -136,9 +123,9 @@ let array_to_fldata_correct
   (u2: unit { array_pred elem_count x } )
 : Lemma
   (ensures (
-    parse_fldata_strong_pred (serialize_list _ () s) array_byte_size x
+    parse_fldata_strong_pred (serialize_list s ()) array_byte_size x
   ))
-= let y = serialize (serialize_list _ () s) x in
+= let y = serialize (serialize_list s ()) x in
   list_length_constant_size_parser_correct p () y
 
 inline_for_extraction
@@ -154,7 +141,7 @@ let array_to_fldata
     fldata_array_precond p array_byte_size elem_count == true
   })
   (x: array t elem_count)
-: Tot (parse_fldata_strong_t (serialize_list _ () s) array_byte_size)
+: Tot (parse_fldata_strong_t (serialize_list s ()) array_byte_size)
 = [@inline_let]
   let (x' : list t) = x in
   [@inline_let]
@@ -195,7 +182,7 @@ let serialize_array
   serialize_synth
     _
     (fldata_to_array s array_byte_size elem_count u)
-    (serialize_fldata_strong (serialize_list _ () s) array_byte_size e)
+    (serialize_fldata_strong (serialize_list s ()) array_byte_size e)
     (array_to_fldata s array_byte_size elem_count u)
     ()
 
@@ -244,12 +231,12 @@ let vldata_to_vlarray_correct
   (elem_count_max: nat)
   (x: list t)
   (u1: unit { vldata_vlarray_precond array_byte_size_min array_byte_size_max p elem_count_min elem_count_max == true } )
-  (u2: unit { parse_bounded_vldata_strong_pred array_byte_size_min array_byte_size_max (serialize_list _ () s) x } )
+  (u2: unit { parse_bounded_vldata_strong_pred array_byte_size_min array_byte_size_max (serialize_list s ()) x } )
 : Lemma
   (ensures (
     vlarray_pred elem_count_min elem_count_max x
   ))
-= let y = serialize (serialize_list _ () s) x in
+= let y = serialize (serialize_list s ()) x in
   let l = L.length x in
   assert (parse (parse_list p ()) y == Correct (x, Seq.length y));
   list_length_constant_size_parser_correct p () y;
@@ -274,7 +261,7 @@ let vldata_to_vlarray
   (u: unit {
     vldata_vlarray_precond array_byte_size_min array_byte_size_max p elem_count_min elem_count_max == true  
   })
-  (x: parse_bounded_vldata_strong_t array_byte_size_min array_byte_size_max (serialize_list _ () s))
+  (x: parse_bounded_vldata_strong_t array_byte_size_min array_byte_size_max (serialize_list s ()))
 : Tot (vlarray t elem_count_min elem_count_max)
 = [@inline_let]
   let x' : list t = x in
@@ -296,7 +283,7 @@ let vldata_to_vlarray_inj
     vldata_vlarray_precond array_byte_size_min array_byte_size_max p elem_count_min elem_count_max == true  
   })
 : Lemma
-  (forall (x1 x2: parse_bounded_vldata_strong_t array_byte_size_min array_byte_size_max (serialize_list _ () s)) .
+  (forall (x1 x2: parse_bounded_vldata_strong_t array_byte_size_min array_byte_size_max (serialize_list s ())) .
     vldata_to_vlarray array_byte_size_min array_byte_size_max s elem_count_min elem_count_max u x1 ==
     vldata_to_vlarray array_byte_size_min array_byte_size_max s elem_count_min elem_count_max u x2 ==>
     x1 == x2)
@@ -312,13 +299,13 @@ let parse_vlarray
   (s: serializer p)
   (elem_count_min: nat)
   (elem_count_max: nat)
+  (e_size_incomplete e_size_invalid e_payload: err)
   (u: unit {
     vldata_vlarray_precond array_byte_size_min array_byte_size_max p elem_count_min elem_count_max == true  
   })
-  (e_size_incomplete e_size_invalid e_payload: err)
 : Tot (parser (parse_bounded_vldata_kind array_byte_size_min array_byte_size_max) (vlarray t elem_count_min elem_count_max) err)
 = vldata_to_vlarray_inj array_byte_size_min array_byte_size_max s elem_count_min elem_count_max u;
-  parse_bounded_vldata_strong array_byte_size_min array_byte_size_max (serialize_list _ () s)
+  parse_bounded_vldata_strong array_byte_size_min array_byte_size_max (serialize_list s ())
    e_size_incomplete e_size_invalid e_payload
   `parse_synth`
   vldata_to_vlarray array_byte_size_min array_byte_size_max s elem_count_min elem_count_max u
@@ -338,9 +325,9 @@ let vlarray_to_vldata_correct
   (u2: unit { vlarray_pred elem_count_min elem_count_max x } )
 : Lemma
   (ensures (
-    parse_bounded_vldata_strong_pred array_byte_size_min array_byte_size_max (serialize_list _ () s) x
+    parse_bounded_vldata_strong_pred array_byte_size_min array_byte_size_max (serialize_list s ()) x
   ))
-= let y = serialize (serialize_list _ () s) x in
+= let y = serialize (serialize_list s ()) x in
   let l = L.length x in
   assert (parse (parse_list p ()) y == Correct (x, Seq.length y));
   list_length_constant_size_parser_correct p () y;
@@ -362,7 +349,7 @@ let vlarray_to_vldata
     vldata_vlarray_precond array_byte_size_min array_byte_size_max p elem_count_min elem_count_max == true  
   })
   (x: vlarray t elem_count_min elem_count_max)
-: Tot (parse_bounded_vldata_strong_t array_byte_size_min array_byte_size_max (serialize_list _ () s))
+: Tot (parse_bounded_vldata_strong_t array_byte_size_min array_byte_size_max (serialize_list s ()))
 = [@inline_let]
   let x' : list t = x in
   [@inline_let]
@@ -399,16 +386,16 @@ let serialize_vlarray
   (s: serializer p)
   (elem_count_min: nat)
   (elem_count_max: nat)
+  (e_size_incomplete e_size_invalid e_payload: err)
   (u: unit {
     vldata_vlarray_precond array_byte_size_min array_byte_size_max p elem_count_min elem_count_max == true  
   })
-  (e_size_incomplete e_size_invalid e_payload: err)
-: Tot (serializer (parse_vlarray array_byte_size_min array_byte_size_max s elem_count_min elem_count_max u e_size_incomplete e_size_invalid e_payload))
+: Tot (serializer (parse_vlarray array_byte_size_min array_byte_size_max s elem_count_min elem_count_max e_size_incomplete e_size_invalid e_payload u))
 = vldata_to_vlarray_inj array_byte_size_min array_byte_size_max s elem_count_min elem_count_max u;
   vlarray_to_vldata_to_vlarray array_byte_size_min array_byte_size_max s elem_count_min elem_count_max u;
   serialize_synth
     _
     (vldata_to_vlarray array_byte_size_min array_byte_size_max s elem_count_min elem_count_max u)
-    (serialize_bounded_vldata_strong array_byte_size_min array_byte_size_max (serialize_list _ () s) e_size_incomplete e_size_invalid e_payload)
+    (serialize_bounded_vldata_strong array_byte_size_min array_byte_size_max (serialize_list s ()) e_size_incomplete e_size_invalid e_payload)
     (vlarray_to_vldata array_byte_size_min array_byte_size_max s elem_count_min elem_count_max u)
     ()
